veric/MemoryPushouts.v
@@ -1,176 +1,8 @@
 Load loadpath.
 Require Import veric.base.
 Require Import Events.
+Require Import veric.MemEvolve.
 
-Lemma mem_inj_id_trans: forall m1 m2 (Inj12: Mem.mem_inj inject_id m1 m2) m3 
-          (Inj23: Mem.mem_inj inject_id m2 m3),Mem.mem_inj inject_id m1 m3.
-Proof. intros.
-  destruct Inj12. rename mi_perm into perm12. rename mi_access into access12. rename mi_memval into memval12.
-  destruct Inj23. rename mi_perm into perm23. rename mi_access into access23. rename mi_memval into memval23.
-  split; intros.
-  (*mi_perm*)
-    apply (perm12 _ _ _ _  _ _ H) in H0. 
-    assert (inject_id b2 = Some (b2, delta)).
-        unfold inject_id in *. inv H. trivial.
-    apply (perm23 _ _ _ _  _ _ H1) in H0.  inv H. inv H1. rewrite Zplus_0_r in H0. assumption.
-  (*mi_access*)
-    apply (access12 _ _ _ _  _ _ H) in H0. 
-    assert (inject_id b2 = Some (b2, delta)).
-        unfold inject_id in *. inv H. trivial.
-    apply (access23 _ _ _ _  _ _ H1) in H0.  inv H. inv H1. rewrite Zplus_0_r in H0. assumption.
-  (*mi_memval*)
-    assert (MV1:= memval12 _ _ _ _  H H0). 
-    assert (inject_id b2 = Some (b2, delta)).
-        unfold inject_id in *. inv H. trivial.
-    assert (R2: Mem.perm m2 b2 ofs Cur Readable).
-        apply (perm12 _ _ _ _  _ _ H) in H0. inv H. rewrite Zplus_0_r in H0. assumption.
-    assert (MV2:= memval23 _ _ _ _  H1 R2).
-    inv H. inv H1.  rewrite Zplus_0_r in *.
-    remember  (ZMap.get ofs (ZMap.get b2 (Mem.mem_contents m2))) as v.
-    destruct v. inv MV1. apply MV2.
-      inv MV1. apply MV2.
-      inv MV2. constructor.
-     inv MV1. inv MV2. inv H3. inv H4. rewrite Int.add_zero. rewrite Int.add_zero.  econstructor. reflexivity. rewrite Int.add_zero.   trivial.
-      inv MV2. inv H3.  rewrite Int.add_zero.   rewrite Int.add_zero in H5. econstructor.
-Qed.
-
-Lemma extends_trans: forall m1 m2 (Ext12: Mem.extends m1 m2) m3 (Ext23: Mem.extends m2 m3), Mem.extends m1 m3.
-Proof. intros. inv Ext12. inv Ext23.
-  split. rewrite mext_next. assumption. eapply mem_inj_id_trans; eauto. 
-Qed.  
-
-Lemma memval_inject_id_refl: forall v, memval_inject inject_id v v. 
-Proof.  destruct v. constructor. constructor. econstructor. reflexivity. rewrite Int.add_zero. trivial. Qed.
-
-Lemma extends_refl: forall m, Mem.extends m m.
-Proof. intros.
-  split. trivial.
-  split; intros. 
-     inv H.  rewrite Zplus_0_r. assumption.
-     inv H.  rewrite Zplus_0_r. assumption.
-     inv H.  rewrite Zplus_0_r. apply memval_inject_id_refl.
-Qed.
-
-Lemma meminj_split_idR: forall j, j = compose_meminj j inject_id.
-Proof. intros. unfold  compose_meminj, inject_id. 
-   apply extensionality. intro b. 
-   remember (j b). 
-   destruct o; trivial. destruct p. rewrite Zplus_0_r. trivial.
-Qed.
-
-Lemma meminj_split_idL: forall j, j = compose_meminj inject_id j.
-Proof. intros. unfold  compose_meminj, inject_id.
-   apply extensionality. intro b.
-   remember (j b). 
-   destruct o; trivial. destruct p. rewrite Zplus_0_l. trivial.  
-Qed.
-
-Goal (*inject_id_refl:*) forall m, Mem.inject inject_id m m.
-Proof.
-  intros. unfold inject_id; split; intros.
-        split; intros; inv H; rewrite Zplus_0_r; trivial.
-        apply memval_inject_id_refl.
-Admitted. (*FAILs*)
-
-Lemma compose_idL: forall f, compose_meminj inject_id f = f.
-Proof. intros. apply extensionality. intros b.
-   unfold compose_meminj.
-   remember (inject_id b).
-   destruct o; inv Heqo. remember (f b). destruct o. destruct  p. rewrite Zplus_0_l. trivial.
-  trivial.
-Qed.
- 
-Lemma compose_idR: forall f, compose_meminj f inject_id = f.
-Proof. intros. apply extensionality. intros b.
-   unfold compose_meminj.
-   remember (f b).
-   destruct o; trivial. destruct  p.
-   remember (inject_id b0).
-   destruct o; inv Heqo0. rewrite Zplus_0_r. trivial.
-Qed.
-
-Lemma extends_inject_compose:
-  forall f m1 m2 m3,
-  Mem.extends m1 m2 -> Mem.inject f m2 m3 -> Mem.inject f m1 m3.
-Proof. intros.
-    inv H. inv mext_inj. inv H0. inv mi_inj.
-    split; intros. 
-         split; intros. 
-             apply (mi_perm _ _ _ _ _ _ (eq_refl _)) in H0. rewrite Zplus_0_r in H0.
-                 apply (mi_perm0 _ _ _ _ _ _ H H0).
-             apply (mi_access _ _ _ _ _ _ (eq_refl _)) in H0. rewrite Zplus_0_r in H0.
-                 apply (mi_access0 _ _ _ _ _ _ H H0).
-             assert (K1:= mi_memval _ _ _ _ (eq_refl _) H0).
-                  apply  (mi_perm _ _ _ _ _ _ (eq_refl _)) in H0. rewrite Zplus_0_r in H0.
-                  assert (K2:= mi_memval0 _ _ _ _ H H0). rewrite Zplus_0_r in K1.
-                  assert (K:= memval_inject_compose _ _ _ _ _ K1 K2).
-                  rewrite compose_idL in K. apply K.
-       apply mi_freeblocks. unfold Mem.valid_block. rewrite <- mext_next. apply H.
-       eapply mi_mappedblocks. apply H.
-        intros b; intros.  apply (mi_perm _ _ _ _ _ _ (eq_refl _)) in H2. rewrite Zplus_0_r in H2. apply (mi_perm _ _ _ _ _ _ (eq_refl _)) in H3. rewrite Zplus_0_r in H3.
-               apply (mi_no_overlap _ _ _ _ _ _ _ _ H H0 H1 H2 H3).
-       apply (mi_perm _ _ _ _ _ _ (eq_refl _)) in H0. rewrite Zplus_0_r in H0.
-                eapply mi_representable. apply H. apply H0.
-Qed.
-
-Lemma inject_extends_compose:
-  forall f m1 m2 m3,
-  Mem.inject f m1 m2 -> Mem.extends m2 m3 -> Mem.inject f m1 m3.
-Proof. intros.
-    inv H. inv mi_inj. inv H0. inv mext_inj.
-    split; intros. 
-         split; intros. 
-             apply (mi_perm _ _ _ _ _ _ H) in H0.
-                 apply (mi_perm0 _ _ _ _ _ _  (eq_refl _)) in H0.  rewrite Zplus_0_r in H0. assumption.
-             apply (mi_access _ _ _ _ _ _ H) in H0.
-                 apply (mi_access0 _ _ _ _ _ _  (eq_refl _)) in H0. rewrite Zplus_0_r in H0. assumption.
-             assert (K1:= mi_memval _ _ _ _ H H0).
-                  apply  (mi_perm _ _ _ _ _ _ H) in H0. 
-                  assert (K2:= mi_memval0 _ _ _ _ (eq_refl _) H0). rewrite Zplus_0_r in K2.
-                  assert (K:= memval_inject_compose _ _ _ _ _ K1 K2).
-                  rewrite compose_idR in K. apply K.
-       apply mi_freeblocks. apply H.
-       unfold Mem.valid_block. rewrite <- mext_next. eapply mi_mappedblocks. apply H.
-        intros b; intros. apply (mi_no_overlap _ _ _ _ _ _ _ _ H H0 H1 H2 H3).
-        eapply mi_representable. apply H. apply H0.
-Qed.
-
-Lemma extends_extends_compose:
-  forall m1 m2 m3,
-  Mem.extends m1 m2 -> Mem.extends m2 m3 -> Mem.extends m1 m3.
-Proof. intros.
-    inv H. inv mext_inj. inv H0. inv mext_inj.
-    split; intros. rewrite mext_next; assumption. 
-    split; intros.
-             apply (mi_perm _ _ _ _ _ _ H) in H0. 
-                 apply (mi_perm0 _ _ _ _ _ _  (eq_refl _)) in H0.  rewrite Zplus_0_r in H0. assumption.
-             apply (mi_access _ _ _ _ _ _ H) in H0.
-                 apply (mi_access0 _ _ _ _ _ _  (eq_refl _)) in H0. rewrite Zplus_0_r in H0. assumption.
-             assert (K1:= mi_memval _ _ _ _ H H0).
-                  apply  (mi_perm _ _ _ _ _ _ H) in H0. 
-                  assert (K2:= mi_memval0 _ _ _ _ (eq_refl _) H0). rewrite Zplus_0_r in K2.
-                  assert (K:= memval_inject_compose _ _ _ _ _ K1 K2).
-                  rewrite compose_idR in K. apply K.
-Qed.
-
-Lemma flatinj_E: forall b b1 b2 delta (H:Mem.flat_inj b b1 = Some (b2, delta)), b2=b1 /\ delta=0 /\ b2 < b.
-Proof. unfold Mem.flat_inj. intros.
-  remember (zlt b1 b).
-  destruct s; inv H. repeat split; trivial.
-Qed.
-
-Lemma flatinj_I: forall bb b, b < bb ->
-               Mem.flat_inj bb b = Some (b, 0).
-Proof. intros. unfold Mem.flat_inj.
-           remember (zlt b bb). destruct s; trivial. exfalso. omega. 
-Qed.
-
-Lemma flatinj_mono: forall b b1 b2 b' delta (F: Mem.flat_inj b1 b = Some (b', delta)),
- Zlt b1 b2 -> Mem.flat_inj b2 b = Some (b', delta).
-Proof. intros.
-   apply flatinj_E in F. destruct F as [? [? ?]]; subst.
-   apply flatinj_I. omega.
-Qed.
 
 Lemma forall_lessdef_refl: forall vals,  Forall2 Val.lessdef vals vals.
 Proof. induction vals; econstructor; trivial. Qed.
@@ -295,7 +127,18 @@ Proof. intros.
   apply IHV.
 Qed.
 
+Lemma val_valid_extends: forall m m2 (Ext12 : Mem.extends m m2) v
+                    (H : val_valid v m), val_valid v m2.
+Proof. intros.
+  destruct v; trivial. simpl in *.
+  eapply (Mem.valid_block_extends _ _ b) in Ext12. eapply Ext12; eassumption.
+Qed.
+
+Lemma mem_unchanged_on_refl: forall m f, mem_unchanged_on f m m.
+Proof. intros. split; intros; trivial. Qed.
+
 Module PUSHOUTS.
+(*
 Require Import veric.Address.
 Require Import veric.sim.
 Definition contents_at (m: mem) (loc: address) : memval := 
@@ -306,9 +149,9 @@ Definition access_at (m: mem) (loc: address) : option permission :=
 
 Definition max_access_at (m: mem) (loc: address) : option permission :=
    ZMap.get (fst loc) (Mem.mem_access m) (snd loc) Max.  
+*)
 
 Section PO_EE.
-Variable m1 m2 m1':mem.
 (*Program Definition PO_EEmem:mem :=
   Mem.mkmem 
         (*content*) 
@@ -325,9 +168,86 @@ Variable m1 m2 m1':mem.
 Check (fun ofs => @ZMap.get memval ofs (ZMap.get b m1'.(Mem.mem_contents))).
                    intros b.*)
 *)
+(*
+Lemma pushout_EE1: forall   m3 m3' v3 (Fwd3: Evolve m3 m3' v3 )
+                 m1 m1' v1 (Fwd1: Evolve m1 m1' v1) m2 (Ext12: Mem.extends m1 m2)
+                 (Ext23: Mem.extends m2 m3) (LD : Val.lessdef v1 v3) 
+                                          (Ext13' : Mem.extends m1' m3')
+                                          (UnchOn3: mem_unchanged_on (loc_out_of_bounds m1) m3 m3'),
+       exists m2',  Evolve m2 m2' v1 /\ Mem.extends m1' m2' /\ mem_unchanged_on (loc_out_of_bounds m1) m2 m2' /\
+                                          Mem.extends m2' m3'.
+Proof. intros m3 m3' v3 Fwd3.
+  induction Fwd3; intros.
+  (*EvolveVal*) rename m into m3. rename v into v3.
+        exists m2. 
+        split. apply EvolveVal. eapply val_valid_extends; eassumption.
+        split. assumption.
+        split. apply mem_unchanged_on_refl.
+        intros m3 m3' v3 Fwd3.
+         induction Fwd3; intros.
+         (*EvolveVal*) assumption.
+         (*EvolveAlloc*) rename m into m3. rename m'' into m3'. rename v into v3.
+                 assert (Mem.nextblock m3 < Mem.nextblock m3').
+                     apply Evolve_nextblock in Fwd3. apply Mem.nextblock_alloc in H0. rewrite H0 in Fwd3.  clear - Fwd3. omega.
+                 assert (Mem.nextblock m3 = Mem.nextblock m3').
+                     clear H0 Fwd3. destruct Ext23. rewrite <- mext_next. 
+                                                destruct Ext12. rewrite <- mext_next0. 
+                                                eapply Ext13'.
+                exfalso. rewrite H2 in H1. clear - H1. omega.
+        (*EvolveStore*) rename m into m3. rename m'' into m3'. rename v into v3. 
+               unfold mem_unchanged_on in UnchOn3. unfold loc_out_of_bounds in UnchOn3.  rewrite <- mext_next0. 
+destruct Ext13'. destruct Ext23. 
+                    split; intros. rewrite <- mext_next0. rewrite mext_next. trivial.
+                            split; intros. destruct mext_inj as [mi_perm12 _ _ ].
+                                      destruct (Fwd3 b2). apply (Mem.valid_block_extends _ _ b2) in Ext23.
+                                      eapply Ext23. inv H0. apply (Mem.perm_valid_block _ _ _ _ _ H1).
+                                     
+ eapply mext_inj0. apply H0. eapply mext_inj.
+ *)
+(*
+Lemma pushout_EE: forall  m1 m1' v1 (Fwd1: Evolve m1 m1' v1) m2 (Ext12: Mem.extends m1 m2),
+       exists m2',  Evolve m2 m2' v1 /\ Mem.extends m1' m2' /\ mem_unchanged_on (loc_out_of_bounds m1) m2 m2' /\
+                          forall m3 m3' v3 (Fwd3: Evolve m3 m3' v3 ) (Ext23: Mem.extends m2 m3) (LD : Val.lessdef v1 v3) 
+                                          (Ext13' : Mem.extends m1' m3')
+                                          (UnchOn3: mem_unchanged_on (loc_out_of_bounds m1) m3 m3'),
+                                          Mem.extends m2' m3'.
+Proof. intros m1 m1' v1 Fwd1.
+  induction Fwd1; intros.
+  (*EvolveVal*) rename m into m1. rename v into v1.
+        exists m2. 
+        split. apply EvolveVal. eapply val_valid_extends; eassumption.
+        split. assumption.
+        split. apply mem_unchanged_on_refl.
+        intros m3 m3' v3 Fwd3.
+         induction Fwd3; intros.
+         (*EvolveVal*) assumption.
+         (*EvolveAlloc*) rename m into m3. rename m'' into m3'. rename v into v3.
+                 assert (Mem.nextblock m3 < Mem.nextblock m3').
+                     apply Evolve_nextblock in Fwd3. apply Mem.nextblock_alloc in H0. rewrite H0 in Fwd3.  clear - Fwd3. omega.
+                 assert (Mem.nextblock m3 = Mem.nextblock m3').
+                     clear H0 Fwd3. destruct Ext23. rewrite <- mext_next. 
+                                                destruct Ext12. rewrite <- mext_next0. 
+                                                eapply Ext13'.
+                exfalso. rewrite H2 in H1. clear - H1. omega.
+        (*EvolveStore*) rename m into m3. rename m'' into m3'. rename v into v3. 
+               unfold mem_unchanged_on in UnchOn3. unfold loc_out_of_bounds in UnchOn3.  rewrite <- mext_next0. 
+destruct Ext13'. destruct Ext23. 
+                    split; intros. rewrite <- mext_next0. rewrite mext_next. trivial.
+                            split; intros. destruct mext_inj as [mi_perm12 _ _ ].
+                                      destruct (Fwd3 b2). apply (Mem.valid_block_extends _ _ b2) in Ext23.
+                                      eapply Ext23. inv H0. apply (Mem.perm_valid_block _ _ _ _ _ H1).
+                                     
+ eapply mext_inj0. apply H0. eapply mext_inj.
+ 
+  
+
+ inv Ext12. unfold mem_forward in Fwd1. inv mext_inj.
+  (*exists PO_EEmem.*)
+*)
+Variable m1 m2 m1':mem.
 Lemma pushout_EE: forall (Ext12: Mem.extends m1 m2) (Fwd1: mem_forward m1 m1'),
        exists m2', mem_forward m2 m2' /\ Mem.extends m1' m2' /\ mem_unchanged_on (loc_out_of_bounds m1) m2 m2' /\
-                          forall m3 (Ext23: Mem.extends m2 m3) m3' (Fwd1: mem_forward m3 m3') 
+                          forall m3 (Ext23: Mem.extends m2 m3) m3' (Fwd3: mem_forward m3 m3') (Ext13' : Mem.extends m1' m3')
                                           (UnchOn3: mem_unchanged_on (loc_out_of_bounds m1) m3 m3'),
                                           Mem.extends m2' m3'.
 Proof. intros. inv Ext12. unfold mem_forward in Fwd1. inv mext_inj.
@@ -335,6 +255,66 @@ Proof. intros. inv Ext12. unfold mem_forward in Fwd1. inv mext_inj.
 Admitted. (*We expect we can iteratively contruct m2' ie walk the blocks (and in the blocks, walk the ofs) to combine
   m1' with m2 pointwise using store operations of the memory model.
   The claim about m3 then (hopefully) follows by an induction on the construction, or is carried around in theproof of the first part*)
+
+Definition pushout_EE_pointwise_contents (m2':mem) := 
+        Mem.nextblock m2' = Mem.nextblock m1' 
+        /\    forall b, if zlt b (Mem.nextblock m1)
+                           then  forall k ofs p,
+                                      (Mem.perm m2' b ofs k p  <->
+                                           (Mem.perm m1' b ofs k p /\ Mem.perm m2 b ofs k p))
+                                      /\
+                                      (Mem.perm m1' b ofs k Readable ->
+                                               (ZMap.get ofs (ZMap.get b m2'.(Mem.mem_contents)) = ZMap.get ofs (ZMap.get b m1'.(Mem.mem_contents))))
+                                      /\  (~ Mem.perm m1' b ofs k Readable -> Mem.perm m2 b ofs k Readable ->
+                                               (ZMap.get ofs (ZMap.get b m2'.(Mem.mem_contents)) = ZMap.get ofs (ZMap.get b m2.(Mem.mem_contents))))
+                           else  (ZMap.get b m2'.(Mem.mem_contents) = ZMap.get b m1'.(Mem.mem_contents) /\
+                                      (forall k ofs p,  Mem.perm m2' b ofs k p = Mem.perm m1' b ofs k p)).
+
+Axiom pushoutEE_exists: exists m2',  pushout_EE_pointwise_contents m2'.
+(*
+Lemma po_EE:  forall (Ext12: Mem.extends m1 m2) (Fwd1: mem_forward m1 m1'),
+       exists m2', mem_forward m2 m2' /\ Mem.extends m1' m2' /\ mem_unchanged_on (loc_out_of_bounds m1) m2 m2' /\
+                          forall m3 (Ext23: Mem.extends m2 m3) m3' (Fwd1: mem_forward m3 m3') 
+                                          (UnchOn3: mem_unchanged_on (loc_out_of_bounds m1) m3 m3'),
+                                          Mem.extends m2' m3'.
+Proof. intros.
+  destruct pushoutEE_exists as [m2' [NB X]]. exists m2'.
+  assert (Fwd2: mem_forward m2 m2').
+            intros b; intros.
+            assert (VB: Mem.valid_block m2' b).
+                     clear X. unfold Mem.valid_block in *. rewrite NB. destruct Ext12. rewrite <- mext_next in H.
+                     eapply (Fwd1 _ H).
+            split; trivial.
+            intros. specialize (X b). 
+                remember (zlt b (Mem.nextblock m1)) as z.
+                destruct z; apply eq_sym in Heqz.
+                   destruct (X Max ofs p) as [P _]; clear X.
+                      apply P. assumption.
+                destruct X as [_ X]. rewrite X in H0.
+                   unfold Mem.valid_block in *. destruct Ext12. rewrite <- mext_next in H.
+                      clear - z H. exfalso. omega.
+  split; trivial.
+  assert (Ext12': Mem.extends m1' m2').
+           split. clear X. rewrite NB. trivial.
+           split; intros. 
+                specialize (X b2). 
+                remember (zlt b2 (Mem.nextblock m1)) as z.
+                destruct z; apply eq_sym in Heqz.
+                   destruct (X k (ofs + 0) p) as [P _]; clear X.
+                      destruct Ext12. destruct mext_inj. specialize (mi_perm _ _ _ ofs k p H).
+                      inv H. rewrite Zplus_0_r in *.
+                      apply P. split; trivial. apply mi_perm. 
+                      destruct (Fwd1 b2 z). apply H1.
+                      destruct Ext12. destruct mext_inj. rewrite <- Zplus_0_r.
+                      eapply (mi_perm b2 b2 0 _ _ _ (eq_refl _) ). H0).
+                destruct X as [_ X]. rewrite X in H0.
+                   unfold Mem.valid_block in *. destruct Ext12. rewrite <- mext_next in H.
+                      clear - z H. exfalso. omega.
+                   unfold mem_forward in Fwd1.
+
+                   admit.
+               *)
+
 End PO_EE.
 
 Section PO_EI.
@@ -363,124 +343,3 @@ exists m2',  Mem.inject j' m1' m2' /\ mem_forward m2 m2' /\
 Admitted.
 End PO_IE.
 End PUSHOUTS.
-
-Module MEM_WD.
-(*memories that do not contain "dangling pointers"*)
-Definition mem_wd m := Mem.inject_neutral (Mem.nextblock m) m.
-
-Lemma mem_wdI: forall m,
-    (forall b ofs  (R:Mem.perm m b ofs Cur Readable),
-                memval_inject  (Mem.flat_inj (Mem.nextblock m)) 
-                                             (ZMap.get ofs (ZMap.get b (Mem.mem_contents m)))
-                                            (ZMap.get ofs (ZMap.get b (Mem.mem_contents m)))) -> mem_wd m.
-Proof. intros.
-  split; intros.
-     apply flatinj_E in  H0. destruct H0 as [? [? ?]]; subst. rewrite Zplus_0_r. trivial. 
-     apply flatinj_E in  H0. destruct H0 as [? [? ?]]; subst. rewrite Zplus_0_r. trivial. 
-     apply flatinj_E in  H0. destruct H0 as [? [? ?]]; subst. rewrite Zplus_0_r.
-        apply H. apply H1.
-Qed.
-        
-Lemma mem_wd_E: forall m, mem_wd m ->  Mem.inject (Mem.flat_inj (Mem.nextblock m)) m m.
-Proof. intros. apply Mem.neutral_inject. apply H. Qed.
-
-Lemma meminj_split_flatinjR: forall j m m' (J:Mem.inject j m' m), mem_wd m -> 
-     j = compose_meminj j (Mem.flat_inj (Mem.nextblock m)).
-Proof. intros. apply mem_wd_E in H.
-   unfold  compose_meminj.
-   apply extensionality. intro b. 
-   remember (j b). 
-   destruct o; trivial. destruct p. unfold Mem.flat_inj in *.
-   remember (zlt b0 (Mem.nextblock m)).
-  destruct s.  rewrite Zplus_0_r. trivial.
-  inv J. apply eq_sym in Heqo. specialize (mi_mappedblocks _ _ _ Heqo).
-               exfalso. unfold Mem.valid_block in mi_mappedblocks. omega.
-Qed.
-
-Lemma meminj_split_flatinjL: forall j m m' (J:Mem.inject j m m'), mem_wd m -> 
-     j = compose_meminj (Mem.flat_inj (Mem.nextblock m)) j.
-Proof. intros. apply mem_wd_E in H.
-   unfold  compose_meminj.
-   apply extensionality. intro b. 
-   unfold Mem.flat_inj in *.
-   remember (zlt b (Mem.nextblock m)).
-  destruct s. remember (j b). destruct o. destruct p.  rewrite Zplus_0_l. trivial. trivial.
-  inv J. apply mi_freeblocks. apply z.
-Qed.
-
-(*Preservation of mem_wd by memory operations*)
-Lemma mem_wd_empty: mem_wd Mem.empty.
-Proof.  apply Mem.empty_inject_neutral. Qed.
-
-Lemma  mem_wd_alloc: forall m b lo hi m' (ALL: Mem.alloc m lo hi = (m',b))
-     (WDm: mem_wd m), mem_wd m'.
-Proof. intros. unfold mem_wd in *.
-  rewrite (Mem.nextblock_alloc _ _ _ _ _ ALL).
-  eapply (Mem.alloc_inject_neutral _ _ _ _ _ _ ALL); try omega.
-  inv WDm. 
-         split; intros. 
-             apply flatinj_E in H. destruct H as [? [? ?]]; subst. rewrite Zplus_0_r. assumption.
-             apply flatinj_E in H. destruct H as [? [? ?]]; subst. rewrite Zplus_0_r. assumption.
-             apply flatinj_E in H. destruct H as [? [? ?]]; subst. rewrite Zplus_0_r.
-                 assert (X: Mem.flat_inj (Mem.nextblock m) b1 = Some (b1, 0)).
-                     apply flatinj_I. apply (Mem.perm_valid_block _ _ _ _ _ H0).
-                  specialize (mi_memval _ _ _ _ X H0). rewrite Zplus_0_r in mi_memval.
-                  eapply memval_inject_incr; try eassumption.
-                       intros bb; intros. eapply flatinj_mono; try eassumption. omega.
-Qed. 
-
-Lemma  mem_wd_drop: forall m b lo hi p m' (DROP: Mem.drop_perm m b lo hi p = Some m')
-     (WDm: mem_wd m), Mem.valid_block m b -> mem_wd m'.
-Proof. intros. unfold mem_wd in *.
-  rewrite (Mem.nextblock_drop _ _ _ _ _ _ DROP).
-  eapply (Mem.drop_inject_neutral _ _ _ _ _ _ _ DROP); trivial.
-Qed.
-  
-Lemma free_neutral: forall (thr : block) (m : mem) (lo hi : Z) (b : block) (m' : Mem.mem')
-  (FREE: Mem.free m b lo hi = Some m'),
-  Mem.inject_neutral thr m -> Mem.inject_neutral thr m'.
-Proof. intros. inv H. 
-  split; intros.
-     apply flatinj_E in H. destruct H as [? [? ?]]; subst. rewrite Zplus_0_r. assumption.
-     apply flatinj_E in H. destruct H as [? [? ?]]; subst. rewrite Zplus_0_r. assumption.
-     apply flatinj_E in H. destruct H as [? [? ?]]; subst. rewrite Zplus_0_r.
-        assert (X: Mem.flat_inj thr b1 = Some (b1,0)). apply flatinj_I. assumption.
-        assert (Y:= Mem.perm_free_3 _ _ _ _ _ FREE _ _ _ _ H0).
-         specialize (mi_memval _ _ _ _ X Y). rewrite Zplus_0_r in *.
-  admit. (*prove that content of m' at that loc is same as in m*)
-Qed.
-
-Lemma mem_wd_free: forall m b lo hi m' (WDm: mem_wd m)
-  (FREE: Mem.free m b lo hi = Some m'), mem_wd m'.
-Proof. intros. unfold mem_wd in *.
-  eapply free_neutral. apply FREE.
-   rewrite (Mem.nextblock_free _ _ _ _ _ FREE). assumption.
-Qed.
-
-(*A value that is (if its a pointer) not dangling wrt m - a condition like this will probably be need to imposed
-on after-external return values (and thus also on the values returned by safely-halted)*)
-Definition val_valid (v:val) (m:mem):Prop := match v with Vptr b ofs => Mem.valid_block m b | _ => True end.
-
-(*In fact valid vals is a slight relaxtion of valid pointers*)
-Lemma valid_ptr_val_valid: forall b ofs m, Mem.valid_pointer m b ofs = true -> val_valid (Vptr b (Int.repr ofs)) m.
-Proof. intros.
-  apply Mem.valid_pointer_nonempty_perm in H. eapply Mem.perm_valid_block. apply H.
-Qed.
-
-Lemma mem_wd_store: forall m b ofs v m' chunk (WDm: mem_wd m)
-  (ST: Mem.store chunk m b ofs v = Some m')
-  (V: val_valid v m), mem_wd m'.
-Proof. intros. unfold mem_wd in *.
-  eapply Mem.store_inject_neutral. apply ST.
-      rewrite (Mem.nextblock_store _ _ _ _ _ _ ST). assumption.
-      assert (X:= Mem.store_valid_access_3 _ _ _ _ _ _ ST).
-          rewrite (Mem.nextblock_store _ _ _ _ _ _ ST). 
-           apply (Mem.valid_access_implies _ _ _ _ _  Nonempty) in X.
-                apply Mem.valid_access_valid_block in X. apply X.
-            constructor.
-      rewrite (Mem.nextblock_store _ _ _ _ _ _ ST). 
-          destruct v. constructor. constructor. constructor.  econstructor. eapply flatinj_I. apply V. rewrite Int.add_zero. trivial.
-Qed.
-
-
-End MEM_WD.
